backend/Linearizeproof.v
@@ -508,18 +508,10 @@ Inductive match_states: LTL.state -> Linear.state -> Prop :=
       match_states (LTL.Block s f sp bb ls m)
                    (Linear.State ts tf sp (linearize_block bb c) ls m)
   | match_states_call:
-<<<<<<< HEAD
-      forall s vf ls m ts,
+      forall s vf ls m ts id,
       list_forall2 match_stackframes s ts ->
-      match_states (LTL.Callstate s vf ls m)
-                   (Linear.Callstate ts vf ls m)
-=======
-      forall s f ls m tf ts id,
-      list_forall2 match_stackframes s ts ->
-      transf_fundef f = OK tf ->
-      match_states (LTL.Callstate s f ls m id)
-                   (Linear.Callstate ts tf ls m id)
->>>>>>> a091c4c
+      match_states (LTL.Callstate s vf ls m id)
+                   (Linear.Callstate ts vf ls m id)
   | match_states_return:
       forall s ls m ts,
       list_forall2 match_stackframes s ts ->
@@ -612,7 +604,6 @@ Proof.
   rewrite (match_parent_locset _ _ STACKS). eauto.
   symmetry; eapply sig_preserved; eauto.
   rewrite (stacksize_preserved _ _ TRF); eauto.
-  rewrite (match_parent_locset _ _ STACKS).
   econstructor; eauto.
 
   (* Lbuiltin *)
@@ -664,11 +655,7 @@ Proof.
   (* internal functions *)
   assert (REACH: (reachable f)!!(LTL.fn_entrypoint f) = true).
     apply reachable_entrypoint.
-<<<<<<< HEAD
   apply functions_translated in FIND as (tf & FIND & MATCH). monadInv MATCH.
-=======
-  monadInv H9.
->>>>>>> a091c4c
   left; econstructor; split.
   apply plus_one. eapply exec_function_internal; eauto.
   rewrite (stacksize_preserved _ _ EQ). eauto.
@@ -676,12 +663,8 @@ Proof.
   econstructor; eauto. simpl. eapply is_tail_add_branch. constructor.
 
   (* external function *)
-<<<<<<< HEAD
   apply functions_translated in FIND as (tf & FIND & MATCH). monadInv MATCH.
   left; econstructor; split.
-=======
-  monadInv H9. left; econstructor; split.
->>>>>>> a091c4c
   apply plus_one. eapply exec_function_external; eauto.
   econstructor; eauto.
 
@@ -709,22 +692,10 @@ Lemma transf_external:
   forall r S', LTL.after_external ge S r S' ->
   exists R', Linear.after_external tge R r R' /\ match_states S' R'.
 Proof.
-<<<<<<< HEAD
   intros S R q HSR Hq. destruct Hq; inv HSR.
   edestruct functions_translated as (tf & FIND & TF); eauto. monadInv TF.
-  split. econstructor; eauto. intros r S' HS'. inv HS'. rewrite H7 in H; inv H.
+  split. econstructor; eauto. intros r S' HS'. inv HS'. rewrite H8 in H; inv H.
   eexists. split; econstructor; eauto.
-=======
-  intros. inversion H.
-  exploit function_ptr_translated; eauto. intros [tf [A B]].
-  exists (Callstate nil tf (Locmap.init Vundef) m0 (prog_main tprog)); split.
-  econstructor; eauto. eapply (Genv.init_mem_transf_partial TRANSF); eauto.
-  rewrite (match_program_main TRANSF).
-  rewrite symbols_preserved. eauto.
-  rewrite <- H3. apply sig_preserved. auto.
-  rewrite (match_program_main TRANSF).
-  constructor. constructor. auto.
->>>>>>> a091c4c
 Qed.
 
 Lemma transf_final_states:
