backend/Mach.v
@@ -249,8 +249,6 @@ Definition extcall_arguments
 
 (** Mach execution states. *)
 
-(** Mach execution states. *)
-
 Inductive stackframe: Type :=
   | Stackframe:
       forall (vf: val)        (**r pointer to calling function *)
@@ -351,22 +349,24 @@ Inductive step: state -> trace -> state -> Prop :=
         E0 (State s f sp c rs' m')
   | exec_Mcall:
       forall s vf sp sig ros c rs m f ra id,
+      let vf1 := ros_address ge ros rs in
+      vf1 = Vptr (Global id) Ptrofs.zero ->
       Genv.find_funct ge vf = Some (Internal f) ->
-      vf = Vptr (Global id) Ptrofs.zero ->
       return_address_offset f c ra ->
       step (State s vf sp (Mcall sig ros :: c) rs m)
         E0 (Callstate (Stackframe vf sp (Val.offset_ptr vf ra) c :: s)
-                      (ros_address ge ros rs) rs m id)
+                      vf1 rs m id)
   | exec_Mtailcall:
       forall s vf stk soff sig ros c rs m f m' m'' id,
+      let vf1 := ros_address ge ros rs in
+      vf1 = Vptr (Global id) Ptrofs.zero ->
       Genv.find_funct ge vf = Some (Internal f) ->
-      vf = Vptr (Global id) Ptrofs.zero ->
       load_stack m (Vptr stk soff) Tptr f.(fn_link_ofs) = Some (parent_sp s) ->
       load_stack m (Vptr stk soff) Tptr f.(fn_retaddr_ofs) = Some (parent_ra s) ->
       Mem.free m stk (Ptrofs.unsigned soff) (Ptrofs.unsigned soff + f.(fn_stacksize)) = Some m' ->
       Mem.return_frame m' = Some m'' ->
       step (State s vf (Vptr stk soff) (Mtailcall sig ros :: c) rs m)
-        E0 (Callstate s (ros_address ge ros rs) rs m'' id)
+        E0 (Callstate s vf1 rs m'' id)
   | exec_Mbuiltin:
       forall s f sp rs m ef args res b vargs t vres rs' m',
       eval_builtin_args ge rs sp m args vargs ->
